add load_rsapss_keys

tests/rsapss-test.c
@@ -14,102 +14,47 @@
 #include "test_helpers.h"
 #include "rsapss_vectors.h"
 
-
-bool hacl_sign(
-  uint32_t modBits,
-  uint8_t *n1,
-  uint32_t pkeyBits,
-  uint8_t *e,
-  uint32_t skeyBits,
-  uint8_t *d,
-  uint32_t msgLen,
-  uint8_t *msg,
-  uint32_t saltLen,
-  uint8_t *salt,
-  uint8_t *sgnt
-)
-{
-  uint32_t nLen = (modBits - (uint32_t)1U) / (uint32_t)64U + (uint32_t)1U;
-  uint32_t eLen = (pkeyBits - (uint32_t)1U) / (uint32_t)64U + (uint32_t)1U;
-  uint32_t dLen = (skeyBits - (uint32_t)1U) / (uint32_t)64U + (uint32_t)1U;
-  uint32_t pkeyLen = nLen + eLen;
-  uint32_t skeyLen = pkeyLen + dLen;
-
-  uint64_t skey[skeyLen];
-  memset(skey, 0U, skeyLen * sizeof (skey[0U]));
-  uint64_t *pkey = skey;
-  uint64_t *nNat = skey;
-  uint64_t *eNat = skey + nLen;
-  uint64_t *dNat = skey + pkeyLen;
-  Hacl_Bignum_Convert_bn_from_bytes_be((modBits - (uint32_t)1U) / (uint32_t)8U + (uint32_t)1U, n1, nNat);
-  Hacl_Bignum_Convert_bn_from_bytes_be((pkeyBits - (uint32_t)1U) / (uint32_t)8U + (uint32_t)1U, e, eNat);
-  Hacl_Bignum_Convert_bn_from_bytes_be((skeyBits - (uint32_t)1U) / (uint32_t)8U + (uint32_t)1U, d, dNat);
-  Hacl_RSAPSS_rsapss_sign(Spec_Hash_Definitions_SHA2_256, modBits, pkeyBits, skeyBits, skey, saltLen, salt, msgLen, msg, sgnt);
-  return 1;
-}
-
-bool hacl_verify(
-  uint32_t modBits,
-  uint8_t *n1,
-  uint32_t pkeyBits,
-  uint8_t *e,
-  uint32_t msgLen,
-  uint8_t *msg,
-  uint32_t saltLen,
-  uint8_t *sgnt
-)
-{
-  uint32_t nLen = (modBits - (uint32_t)1U) / (uint32_t)64U + (uint32_t)1U;
-  uint32_t eLen = (pkeyBits - (uint32_t)1U) / (uint32_t)64U + (uint32_t)1U;
-  uint32_t pkeyLen = nLen + eLen + nLen;
-
-  uint64_t pkey[pkeyLen];
-  memset(pkey, 0U, pkeyLen * sizeof pkey[0U]);
-  uint64_t *nNat = pkey;
-  uint64_t *eNat = pkey + nLen;
-  Hacl_Bignum_Convert_bn_from_bytes_be((modBits - (uint32_t)1U) / (uint32_t)8U + (uint32_t)1U, n1, nNat);
-  Hacl_Bignum_Convert_bn_from_bytes_be((pkeyBits - (uint32_t)1U) / (uint32_t)8U + (uint32_t)1U, e, eNat);
-
-  bool verify_sgnt = Hacl_RSAPSS_rsapss_verify(Spec_Hash_Definitions_SHA2_256, modBits, pkeyBits, pkey, saltLen, sgnt, msgLen, msg);
-  return verify_sgnt;
-}
-
 bool print_result(uint32_t len, uint8_t* comp, uint8_t* exp) {
   return compare_and_print(len, comp, exp);
 }
 
 bool print_test(
   uint32_t modBits,
-  uint8_t *n1,
-  uint32_t pkeyBits,
-  uint8_t *e,
-  uint32_t skeyBits,
-  uint8_t *d,
+  uint32_t eBits,
+  uint32_t dBits,
+  uint8_t *nb,
+  uint8_t *eb,
+  uint8_t *db,
   uint32_t msgLen,
   uint8_t *msg,
   uint32_t saltLen,
   uint8_t *salt,
   uint8_t *sgnt_expected
 ){
-  uint32_t nTLen = (modBits - (uint32_t)1U) / (uint32_t)8U + (uint32_t)1U;
-  uint8_t sgnt[nTLen];
-  memset(sgnt, 0U, nTLen * sizeof (sgnt[0U]));
-  bool ok = hacl_sign(modBits, n1, pkeyBits, e, skeyBits, d, msgLen, msg, saltLen, salt, sgnt);
+  uint32_t nbLen = (modBits - (uint32_t)1U) / (uint32_t)8U + (uint32_t)1U;
+  uint8_t sgnt[nbLen];
+  memset(sgnt, 0U, nbLen * sizeof (sgnt[0U]));
+
+  uint64_t *pkey = Hacl_RSAPSS_new_rsapss_load_pkey(modBits, eBits, nb, eb);
+  uint64_t *skey = Hacl_RSAPSS_new_rsapss_load_skey(modBits, eBits, dBits, nb, eb, db);
+
+
+  Hacl_RSAPSS_rsapss_sign(Spec_Hash_Definitions_SHA2_256, modBits, eBits, dBits, skey, saltLen, salt, msgLen, msg, sgnt);
   printf("RSAPSS sign Result:\n");
-  ok = ok && print_result(nTLen, sgnt, sgnt_expected);
+  bool ok = print_result(nbLen, sgnt, sgnt_expected);
 
   printf("RSAPSS verify Result:\n");
-  bool ver = hacl_verify(modBits, n1, pkeyBits, e, msgLen, msg, saltLen, sgnt);
+  bool ver = Hacl_RSAPSS_rsapss_verify(Spec_Hash_Definitions_SHA2_256, modBits, eBits, pkey, saltLen, sgnt, msgLen, msg);
   if (ver) printf("Success!\n");
   ok = ok && ver;
   return ok;
 }
 
-int main() {
 
+int main() {
   bool ok = true;
   for (int i = 0; i < sizeof(vectors)/sizeof(rsapss_test_vector); ++i) {
-    ok &= print_test(vectors[i].modBits,vectors[i].n,vectors[i].eBits,vectors[i].e,vectors[i].dBits,vectors[i].d,
+    ok &= print_test(vectors[i].modBits,vectors[i].eBits,vectors[i].dBits,vectors[i].n,vectors[i].e,vectors[i].d,
 		     vectors[i].msgLen,vectors[i].msg,vectors[i].saltLen,vectors[i].salt,vectors[i].sgnt_expected);
   }
 
