code/rsapss/Hacl.RSAPSS.fst
@@ -3,13 +3,23 @@ module Hacl.RSAPSS
 module S = Spec.RSAPSS
 module Hash = Spec.Agile.Hash
 
+module IR = Hacl.Impl.RSAPSS
+
 #reset-options "--z3rlimit 50 --fuel 0 --ifuel 0"
 
-val rsapss_sign: a:Hash.algorithm{S.hash_is_supported a} -> Hacl.Impl.RSAPSS.rsapss_sign_st a
+val rsapss_sign: a:Hash.algorithm{S.hash_is_supported a} -> IR.rsapss_sign_st a
 let rsapss_sign a modBits eBits dBits skey sLen salt msgLen msg sgnt =
-  Hacl.Impl.RSAPSS.rsapss_sign a modBits eBits dBits skey sLen salt msgLen msg sgnt
+  IR.rsapss_sign a modBits eBits dBits skey sLen salt msgLen msg sgnt
 
-
-val rsapss_verify: a:Hash.algorithm{S.hash_is_supported a} -> Hacl.Impl.RSAPSS.rsapss_verify_st a
+val rsapss_verify: a:Hash.algorithm{S.hash_is_supported a} -> IR.rsapss_verify_st a
 let rsapss_verify a modBits eBits pkey sLen sgnt msgLen msg =
-  Hacl.Impl.RSAPSS.rsapss_verify a modBits eBits pkey sLen sgnt msgLen msg
+  IR.rsapss_verify a modBits eBits pkey sLen sgnt msgLen msg
+
+
+val new_rsapss_load_pkey: IR.new_rsapss_load_pkey_st
+let new_rsapss_load_pkey r modBits eBits nb eb =
+  IR.new_rsapss_load_pkey r modBits eBits nb eb
+
+val new_rsapss_load_skey: IR.new_rsapss_load_skey_st
+let new_rsapss_load_skey r modBits eBits dBits nb eb db =
+  IR.new_rsapss_load_skey r modBits eBits dBits nb eb db
